theories/Syntax/UnOps.v
@@ -175,6 +175,9 @@ Module uop.
       | negate              => bv.negate
       end.
 
+    Definition evalRel {σ1 σ2 : Ty} (op : UnOp σ1 σ2) : RelVal σ1 -> RelVal σ2 :=
+      liftUnOp (eval op).
+
   End WithTypeDef.
   #[export] Existing Instance eq_dec_unop.
 
